wrap proof for languages containing the empty word. Change theorem interface.

Roos/Chomsky_Schuetzenberger.thy
@@ -1,5 +1,5 @@
 theory Chomsky_Schuetzenberger
-  imports "../CFG" "../CFL" "../Parse_Tree" "Finite_Automata_Not_HF" "$AFP/Regular-Sets/Regexp_Constructions"
+  imports "../CFG" "../CFL" "../Parse_Tree" "Finite_Automata_Not_HF" "$AFP/Wlog/Wlog" "../Stimpfle/CNF"
 begin
 
 text \<open>This file contains all the constructions needed for the chomsky-schuetzenberger theorem.
@@ -1285,7 +1285,7 @@ lemma Re_sym_imp_Re_for_tm[intro, dest]: \<open>(map Tm x) \<in> Re_sym A \<Long
 
 text\<open>Definition of monoid-homomorphism where multiplication is that of words.\<close>
 definition hom :: \<open>('c list \<Rightarrow> 'd list) \<Rightarrow> bool\<close> where
-  \<open>hom h = (\<forall>a b. h (a@b) = (h a) @ h (b))\<close>
+  \<open>hom h = ((\<forall>a b. h (a@b) = (h a) @ h (b)) \<and> h [] = [])\<close>
 
 
 text\<open>helper function for the definition of \<open>h\<close>\<close>
@@ -2991,62 +2991,43 @@ qed
 
 
 
-
-
-
-(* 
-text\<open>TODO: only assume Type 2 for L and finite productions somehow, then obtain a finite CNF grammar in the proof. Use (and adapt CNF_existence).\<close>
-text\<open>Existence of chomsky normal form. Doesn't forbid the start symbol on the right though, so it's techinally even weaker.\<close>
-lemma CNF_existence :
-  assumes \<open>CFL.cfl TYPE('a) L\<close>
-  shows \<open>\<exists>P S::'a. L = Lang P S \<and> (\<forall>p \<in> P. CNF_rule p)\<close> (* TODO start symbol not on the right side*)
-  sorry
-
-*)
-
-
 section\<open>The Theorem\<close>
 
 
-declare [[show_types]]
-
-text\<open>The chomsky-scheutzenberger theorem that we want to prove.\<close>
+text\<open>The constructive version of the Theorem, for a grammar already in CNF\<close>
 lemma chomsky_schuetzenberger_constr:
-  fixes L::\<open>'t list set\<close> and  P :: \<open>('n, 't) Prods\<close> and S::"'n"
-  assumes \<open>L = Lang P S\<close> and P_CNF: \<open>(\<forall>p \<in> P. CNF_rule p)\<close> and \<open>finite P\<close>
-  shows \<open>regular ((brackets P) \<inter> Re S) \<and> L = image the_hom( ( (brackets P) \<inter> Re S) \<inter> (dyck_language(P \<times> {One, Two}) ) ) \<and> hom (the_hom:: (bracket \<times> ('n \<times> ('n, 't) sym list) \<times> version) list
-   \<Rightarrow> 't list)\<close>
+  fixes P :: \<open>('n::infinite, 't) Prods\<close> and S::"'n"
+  defines \<open>L \<equiv> CFG.Lang P S\<close>
+  assumes finite: \<open>finite P\<close> and P_CNF: \<open>CNF P\<close>
+  shows \<open>regular ((brackets P) \<inter> Re S) \<and> L = image the_hom( ( (brackets P) \<inter> Re S) \<inter> (dyck_language(P \<times> {One, Two}) ) ) \<and> hom (the_hom:: (bracket \<times> ('n \<times> ('n, 't) sym list) \<times> version) list \<Rightarrow> 't list)\<close>
 proof -
-  (* have \<open>\<exists>P S::'n. L = Lang P S \<and> (\<forall>p \<in> P. CNF_rule p)\<close> using \<open>cfl TYPE('n) L\<close> CNF_existence by auto
-  then obtain P and S::'n where \<open>L = Lang P S\<close> and P_CNF: \<open>(\<forall>p \<in> P. CNF_rule p)\<close> by blast *)
-
   define \<Gamma> where \<open>\<Gamma> = P \<times> {One, Two}\<close>
   define P' where \<open>P' = image transform_production P\<close>
   define L' where \<open>L' = Lang P' S\<close>
   define h where \<open>h = (the_hom::(bracket \<times> ('n \<times> ('n, 't) sym list) \<times> version) list \<Rightarrow> 't list)\<close>
   define h_ext where \<open>h_ext = (the_hom_ext::('n, bracket \<times> ('n,'t) prod \<times> version ) sym list \<Rightarrow> ('n,'t) sym list)\<close>
 
+  have P_CNF': \<open>(\<forall>p \<in> P. CNF_rule p)\<close> using P_CNF unfolding CNF.CNF_def CNF_rule_def by fastforce 
 
   have \<open>\<forall>A. \<forall>x. P' \<turnstile> [Nt A] \<Rightarrow>* (map Tm x) \<longleftrightarrow> x \<in> (dyck_language \<Gamma>) \<inter> (Re A)\<close> (* This is the hard part of the proof - the local lemma in the textbook *)
   proof-
 
-    have \<open>\<And>A x.  P' \<turnstile> [Nt A] \<Rightarrow>* x \<Longrightarrow> bal_tm x \<and> rhs_in_if x (P \<times> {One, Two})\<close> by (simp add: P'_bal P'_def P_CNF)
+    have \<open>\<And>A x.  P' \<turnstile> [Nt A] \<Rightarrow>* x \<Longrightarrow> bal_tm x \<and> rhs_in_if x (P \<times> {One, Two})\<close> by (simp add: P'_bal P'_def P_CNF')
     then have hr1: \<open>\<And>A x. (P' \<turnstile> [Nt A] \<Rightarrow>* (map Tm x) \<Longrightarrow> x \<in> dyck_language \<Gamma>)\<close> using \<Gamma>_def by (meson dyck_languageI_tm)
 
 
-    have \<open>\<And>A x.  P' \<turnstile> [Nt A] \<Rightarrow>* x \<Longrightarrow> x \<in> Re_sym A\<close> using P'_imp_Re using P'_def P_CNF by fastforce
+    have \<open>\<And>A x.  P' \<turnstile> [Nt A] \<Rightarrow>* x \<Longrightarrow> x \<in> Re_sym A\<close> using P'_imp_Re using P'_def P_CNF' by fastforce
     then have hr2: \<open>\<And>A x.  P' \<turnstile> [Nt A] \<Rightarrow>* map Tm x \<Longrightarrow> x \<in> Re A\<close> by blast
 
-    have rr: \<open>\<And>A x.  x \<in> (dyck_language \<Gamma>) \<inter> (Re A) \<Longrightarrow> (P' \<turnstile> [Nt A] \<Rightarrow>* (map Tm x)) \<close> using Re_imp_P' by (metis P'_def P_CNF \<Gamma>_def inf_sup_aci(1))
+    have rr: \<open>\<And>A x.  x \<in> (dyck_language \<Gamma>) \<inter> (Re A) \<Longrightarrow> (P' \<turnstile> [Nt A] \<Rightarrow>* (map Tm x)) \<close> using Re_imp_P' by (metis P'_def P_CNF' \<Gamma>_def inf_sup_aci(1))
 
 
     show ?thesis using hr1 hr2 rr by (meson Int_iff)
 
   qed
 
+  then have \<open>L' = (dyck_language \<Gamma>) \<inter> (Re S)\<close> by (auto simp add: CFG.Lang_def L'_def)
 
-
-  then have \<open>L' = (dyck_language \<Gamma>) \<inter> (Re S)\<close> by (metis CFL_Lang_eq_CFG_Lang CFL_Lang_if_derives L'_def derives_if_CFL_Lang inf_absorb2 inf_commute subsetI)
   then have \<open>image h ((dyck_language \<Gamma>) \<inter> (Re S)) =  image h L'\<close> by simp
   also have \<open>... = Lang P S\<close>
   proof(standard)
@@ -3055,7 +3036,7 @@ proof -
       fix w'
       assume \<open>w' \<in> L'\<close>
       with L'_def have \<open>w' \<in> Lang P' S\<close> by simp
-      then have \<open>P' \<turnstile> [Nt S] \<Rightarrow>* map Tm w'\<close> by (simp add: CFL_Lang_eq_CFG_Lang derives_if_CFL_Lang)
+      then have \<open>P' \<turnstile> [Nt S] \<Rightarrow>* map Tm w'\<close> by (simp add: CFG.Lang_def)
       then obtain n where \<open>P' \<turnstile> [Nt S] \<Rightarrow>(n) map Tm w'\<close> by (metis rtranclp_power)
       then have \<open>P \<turnstile> [Nt S] \<Rightarrow>* h_ext (map Tm w')\<close> 
       proof(induction rule: deriven_induct)
@@ -3064,7 +3045,7 @@ proof -
       next
         case (Suc n u A v x')
         from \<open>(A, x') \<in> P'\<close> obtain \<pi> where \<open>\<pi> \<in> P\<close> and transf_\<pi>_def: \<open>(transform_production \<pi>) = (A, x')\<close> using P'_def by auto
-        moreover have \<open>CNF_rule \<pi>\<close> using P_CNF \<open>\<pi> \<in> P\<close> by auto
+        moreover have \<open>CNF_rule \<pi>\<close> using P_CNF' \<open>\<pi> \<in> P\<close> by auto
         ultimately obtain x where \<pi>_def: \<open>\<pi> = (A, x)\<close> using transform_production_CNF by (smt (verit, del_insts) CNF_rule_def Pair_inject Chomsky_Schuetzenberger.transform_production.simps(1,2))
         have \<open>hom h_ext\<close> unfolding hom_def h_ext_def the_hom_ext.simps by simp
         then have \<open>h_ext (u @ [Nt A] @ v) = h_ext u @ h_ext [Nt A] @ h_ext v\<close> using hom_def by (metis (no_types, lifting))
@@ -3080,14 +3061,14 @@ proof -
         with \<open> P \<turnstile> [Nt S] \<Rightarrow>* h_ext u @ x @ h_ext v\<close> have \<open> P \<turnstile> [Nt S] \<Rightarrow>* h_ext u @ h_ext x' @ h_ext v\<close> by simp
         then show ?case by (metis \<open>hom h_ext\<close> hom_def)
       qed
-      then show \<open>h w' \<in> Lang P S\<close> using h_eq_h_ext h_ext_def by (metis CFL_Lang_eq_CFG_Lang CFL_Lang_if_derives h_def)
+      then show \<open>h w' \<in> Lang P S\<close> using h_eq_h_ext h_ext_def by (metis CFG.Lang_def h_def mem_Collect_eq)
     qed
     then show \<open> h ` L' \<subseteq> Lang P S\<close> by (simp add: image_subsetI)
 
   next
     have \<open>\<And>w. (w  \<in> Lang P S \<Longrightarrow> \<exists>w' \<in> L'. w = h w')\<close> 
     proof-
-      have \<open>\<And>w. (w \<in> Ders P S \<Longrightarrow> \<exists>w' \<in> Ders P' S. w = h_ext w')\<close> using transfer_parse_tree by (metis P'_def P_CNF h_ext_def)
+      have \<open>\<And>w. (w \<in> Ders P S \<Longrightarrow> \<exists>w' \<in> Ders P' S. w = h_ext w')\<close> using transfer_parse_tree by (metis P'_def P_CNF' h_ext_def)
       then show \<open>\<And>w. (w  \<in> Lang P S \<Longrightarrow> \<exists>w' \<in> L'. w = h w')\<close>
       proof(goal_cases)
         case (1 w)
@@ -3102,7 +3083,7 @@ proof -
     then show \<open>Lang P S \<subseteq> h ` L'\<close> by auto 
   qed
 
-  also have \<open>... = L\<close> by (simp add: \<open>L = Lang P S\<close>)
+  also have \<open>... = L\<close> by (simp add: L_def)
   finally have \<open>image h ((dyck_language \<Gamma>) \<inter> (Re S)) = L\<close> by auto
 
   moreover have \<open>((dyck_language \<Gamma>) \<inter> ((brackets P) \<inter> Re S)) = ((dyck_language \<Gamma>) \<inter> (Re S))\<close>
@@ -3121,120 +3102,51 @@ qed
 
 
 
-
-
-
-
-
-
-
-
-text\<open>The chomsky-scheutzenberger theorem that we want to prove.\<close>
-lemma chomsky_schuetzenberger :
-  fixes L::\<open>'t list set\<close> and  P :: \<open>('n, 't) Prods\<close>
-  assumes \<open>L = Lang P S\<close> and P_CNF: \<open>(\<forall>p \<in> P. CNF_rule p)\<close> and \<open>finite P\<close> \<comment> \<open> TODO: only assume Type 2 for L and finite productions somehow, then obtain a finite CNF grammar in the proof. Use (and adapt CNF_existence).  \<close>
-    \<comment> \<open>TODO2, with cnf stuff we need to wrap the proof for Languages containing \<epsilon>.\<close>
+text\<open>The theorem, but only for languages not containing \<open>\<epsilon>\<close> \<close>
+lemma chomsky_schuetzenberger_not_empty:
+  fixes P :: \<open>('n::infinite, 't) Prods\<close> and S::"'n"
+  defines \<open>L \<equiv> CFG.Lang P S - {[]}\<close>
+  assumes finite: \<open>finite P\<close>
   shows \<open>\<exists>(R::(bracket \<times> ('n \<times> ('n, 't) sym list) \<times> version) list set) h \<Gamma>. (regular R) \<and> (L = image h (R \<inter> dyck_language \<Gamma>)) \<and> hom h\<close>
 proof -
-  (* have \<open>\<exists>P S::'n. L = Lang P S \<and> (\<forall>p \<in> P. CNF_rule p)\<close> using \<open>cfl TYPE('n) L\<close> CNF_existence by auto
-  then obtain P and S::'n where \<open>L = Lang P S\<close> and P_CNF: \<open>(\<forall>p \<in> P. CNF_rule p)\<close> by blast *)
-
-  define \<Gamma> where \<open>\<Gamma> = P \<times> {One, Two}\<close>
-  define P' where \<open>P' = image transform_production P\<close>
-  define L' where \<open>L' = Lang P' S\<close>
-  define h where \<open>h = (the_hom::(bracket \<times> ('n \<times> ('n, 't) sym list) \<times> version) list \<Rightarrow> 't list)\<close>
-  define h_ext where \<open>h_ext = (the_hom_ext::('n, bracket \<times> ('n,'t) prod \<times> version ) sym list \<Rightarrow> ('n,'t) sym list)\<close>
-
-
-  have \<open>\<forall>A. \<forall>x. P' \<turnstile> [Nt A] \<Rightarrow>* (map Tm x) \<longleftrightarrow> x \<in> (dyck_language \<Gamma>) \<inter> (Re A)\<close> (* This is the hard part of the proof - the local lemma in the textbook *)
-  proof-
-
-    have \<open>\<And>A x.  P' \<turnstile> [Nt A] \<Rightarrow>* x \<Longrightarrow> bal_tm x \<and> rhs_in_if x (P \<times> {One, Two})\<close> by (simp add: P'_bal P'_def P_CNF)
-    then have hr1: \<open>\<And>A x. (P' \<turnstile> [Nt A] \<Rightarrow>* (map Tm x) \<Longrightarrow> x \<in> dyck_language \<Gamma>)\<close> using \<Gamma>_def by (meson dyck_languageI_tm)
-
-
-    have \<open>\<And>A x.  P' \<turnstile> [Nt A] \<Rightarrow>* x \<Longrightarrow> x \<in> Re_sym A\<close> using P'_imp_Re using P'_def P_CNF by fastforce
-    then have hr2: \<open>\<And>A x.  P' \<turnstile> [Nt A] \<Rightarrow>* map Tm x \<Longrightarrow> x \<in> Re A\<close> by blast
-
-    have rr: \<open>\<And>A x.  x \<in> (dyck_language \<Gamma>) \<inter> (Re A) \<Longrightarrow> (P' \<turnstile> [Nt A] \<Rightarrow>* (map Tm x)) \<close> using Re_imp_P' by (metis P'_def P_CNF \<Gamma>_def inf_sup_aci(1))
-
-
-    show ?thesis using hr1 hr2 rr by (meson Int_iff)
-
-  qed
-
-
-
-  then have \<open>L' = (dyck_language \<Gamma>) \<inter> (Re S)\<close> by (metis CFL_Lang_eq_CFG_Lang CFL_Lang_if_derives L'_def derives_if_CFL_Lang inf_absorb2 inf_commute subsetI)
-  then have \<open>image h ((dyck_language \<Gamma>) \<inter> (Re S)) =  image h L'\<close> by simp
-  also have \<open>... = Lang P S\<close>
-  proof(standard)
-    have \<open>\<And>w'. (w'  \<in> L' \<Longrightarrow> h w' \<in> Lang P S)\<close>
-    proof-
-      fix w'
-      assume \<open>w' \<in> L'\<close>
-      with L'_def have \<open>w' \<in> Lang P' S\<close> by simp
-      then have \<open>P' \<turnstile> [Nt S] \<Rightarrow>* map Tm w'\<close> by (simp add: CFL_Lang_eq_CFG_Lang derives_if_CFL_Lang)
-      then obtain n where \<open>P' \<turnstile> [Nt S] \<Rightarrow>(n) map Tm w'\<close> by (metis rtranclp_power)
-      then have \<open>P \<turnstile> [Nt S] \<Rightarrow>* h_ext (map Tm w')\<close> 
-      proof(induction rule: deriven_induct)
-        case 0
-        then show ?case unfolding h_ext_def the_hom_ext.simps by simp
-      next
-        case (Suc n u A v x')
-        from \<open>(A, x') \<in> P'\<close> obtain \<pi> where \<open>\<pi> \<in> P\<close> and transf_\<pi>_def: \<open>(transform_production \<pi>) = (A, x')\<close> using P'_def by auto
-        moreover have \<open>CNF_rule \<pi>\<close> using P_CNF \<open>\<pi> \<in> P\<close> by auto
-        ultimately obtain x where \<pi>_def: \<open>\<pi> = (A, x)\<close> using transform_production_CNF by (smt (verit, del_insts) CNF_rule_def Pair_inject Chomsky_Schuetzenberger.transform_production.simps(1,2))
-        have \<open>hom h_ext\<close> unfolding hom_def h_ext_def the_hom_ext.simps by simp
-        then have \<open>h_ext (u @ [Nt A] @ v) = h_ext u @ h_ext [Nt A] @ h_ext v\<close> using hom_def by (metis (no_types, lifting))
-        then have \<open> P \<turnstile> [Nt S] \<Rightarrow>* h_ext u @ h_ext [Nt A] @ h_ext v\<close> using local.Suc.IH by auto
-        then have \<open> P \<turnstile> [Nt S] \<Rightarrow>* h_ext u @ [Nt A] @ h_ext v\<close> unfolding h_ext_def by simp
-        then have \<open> P \<turnstile> [Nt S] \<Rightarrow>* h_ext u @ x @ h_ext v\<close> using \<pi>_def \<open>\<pi> \<in> P\<close> derive.intros by (metis Transitive_Closure.rtranclp.rtrancl_into_rtrancl)
-
-        have \<open>h_ext x' = h_ext (snd (transform_production \<pi>))\<close> by (simp add: transf_\<pi>_def)
-        also have \<open>... = snd \<pi>\<close> using \<open>CNF_rule \<pi>\<close> h_ext_def hom_ext_inv by blast
-        also have \<open>... = x\<close> by (simp add: \<pi>_def)
-        finally have \<open>h_ext x' = x\<close> by simp
-
-        with \<open> P \<turnstile> [Nt S] \<Rightarrow>* h_ext u @ x @ h_ext v\<close> have \<open> P \<turnstile> [Nt S] \<Rightarrow>* h_ext u @ h_ext x' @ h_ext v\<close> by simp
-        then show ?case by (metis \<open>hom h_ext\<close> hom_def)
-      qed
-      then show \<open>h w' \<in> Lang P S\<close> using h_eq_h_ext h_ext_def by (metis CFL_Lang_eq_CFG_Lang CFL_Lang_if_derives h_def)
-    qed
-    then show \<open> h ` L' \<subseteq> Lang P S\<close> by (simp add: image_subsetI)
-
-  next
-    have \<open>\<And>w. (w  \<in> Lang P S \<Longrightarrow> \<exists>w' \<in> L'. w = h w')\<close> 
-    proof-
-      have \<open>\<And>w. (w \<in> Ders P S \<Longrightarrow> \<exists>w' \<in> Ders P' S. w = h_ext w')\<close> using transfer_parse_tree by (metis P'_def P_CNF h_ext_def)
-      then show \<open>\<And>w. (w  \<in> Lang P S \<Longrightarrow> \<exists>w' \<in> L'. w = h w')\<close>
-      proof(goal_cases)
-        case (1 w)
-        then have \<open>(map Tm w) \<in> Ders P S\<close> using Lang_Ders imageI by fastforce
-        then obtain w' where w'_def: \<open>w' \<in> Ders P' S\<close> \<open>(map Tm w) = h_ext w'\<close> using \<open>\<And>w. w \<in> Ders P S \<Longrightarrow> \<exists>w'\<in> Ders P' S. w = h_ext w'\<close>[of \<open>map Tm w\<close>] by blast 
-        moreover obtain w'' where \<open>w' = map Tm w''\<close> using w'_def by (metis h_ext_def the_hom_ext_tms_inj)
-        then have \<open>w = h w''\<close> using h_eq_h_ext2 h_def h_ext_def by (metis h_eq_h_ext w'_def(2))
-        moreover have \<open>w'' \<in> L'\<close> using \<open>w' \<in> Ders P' S\<close> by (metis DersD \<open>L' = dyck_language \<Gamma> \<inter> Re S\<close> \<open>\<forall>A. \<forall>x. P' \<turnstile> [Nt A] \<Rightarrow>* (map Tm x) \<longleftrightarrow> x \<in> (dyck_language \<Gamma>) \<inter> (Re A)\<close> \<open>w' = map Tm w''\<close>)
-        ultimately show ?case by auto
-      qed
-    qed
-    then show \<open>Lang P S \<subseteq> h ` L'\<close> by auto 
-  qed
-
-  also have \<open>... = L\<close> by (simp add: \<open>L = Lang P S\<close>)
-  finally have \<open>image h ((dyck_language \<Gamma>) \<inter> (Re S)) = L\<close> by auto
-
-  moreover have \<open>((dyck_language \<Gamma>) \<inter> ((brackets P) \<inter> Re S)) = ((dyck_language \<Gamma>) \<inter> (Re S))\<close>
-  proof
-    show \<open>dyck_language \<Gamma> \<inter> ((brackets P) \<inter> Re S) \<subseteq> dyck_language \<Gamma> \<inter> Re S\<close> by blast
-  next
-    show \<open>dyck_language \<Gamma> \<inter> Re S \<subseteq> dyck_language \<Gamma> \<inter> ((brackets P) \<inter> Re S)\<close> using \<Gamma>_def dyck_lang_imp_star_brackets by auto
-  qed
-  moreover have hom: \<open>hom h\<close> by (simp add: h_def hom_def)
-  moreover from \<open>finite P\<close> have \<open>regular ((brackets P) \<inter> Re S)\<close> using regular_Re_inter by fast
-  ultimately have \<open>regular ((brackets P) \<inter> Re S) \<and> L = image h (((brackets P) \<inter> Re S) \<inter> (dyck_language \<Gamma>)) \<and> hom h\<close> by (simp add: inf_commute)
-  then show ?thesis by blast
+  define h where \<open>h = (the_hom:: (bracket \<times> ('n \<times> ('n, 't) sym list) \<times> version) list \<Rightarrow> 't list)\<close>
+  obtain ps where ps_def: \<open>set ps = P\<close> using finite finite_list by auto
+  from cnf_exists obtain ps' where ps'_CNF: \<open>CNF(set ps')\<close> and lang_ps_eq_lang_ps': \<open>CFG.lang ps' S = CFG.lang ps S - {[]}\<close> by blast
+  then have \<open>finite( set ps')\<close> and \<open>CNF( set ps')\<close> by auto
+  then have \<open>regular (brackets (set ps') \<inter> Re S) \<and> CFG.lang ps' S = h ` (brackets (set ps') \<inter> Re S \<inter> dyck_language (set ps' \<times> {One, Two})) \<and> hom h\<close> using chomsky_schuetzenberger_constr[OF \<open>finite( set ps')\<close> \<open>CNF( set ps')\<close>, of S] using h_def by fastforce
+  moreover have  \<open>CFG.lang ps' S = L - {[]}\<close> unfolding lang_ps_eq_lang_ps' using L_def ps_def by blast
+  ultimately have eq: \<open>regular (brackets (set ps') \<inter> Re S) \<and> L - {[]} = h ` (brackets (set ps') \<inter> Re S \<inter> dyck_language (set ps' \<times> {One, Two})) \<and> hom h\<close> by presburger
+  then show ?thesis using L_def by auto
 qed
+
+
+
+
+
+
+
+
+text\<open>The chomsky-scheutzenberger theorem that we really want to prove.\<close>
+lemma chomsky_schuetzenberger:
+  fixes P :: \<open>('n::infinite, 't) Prods\<close> and S::"'n"
+  defines \<open>L \<equiv> CFG.Lang P S\<close>
+  assumes finite: \<open>finite P\<close>
+  shows \<open>\<exists>(R::(bracket \<times> ('n \<times> ('n, 't) sym list) \<times> version) list set) h \<Gamma>.  (regular R) \<and> (L = image h (R \<inter> dyck_language \<Gamma>)) \<and> hom h\<close>
+proof(cases \<open>[] \<in> L\<close>)
+  case False
+  then show ?thesis by (metis Diff_empty Diff_insert0 L_def chomsky_schuetzenberger_not_empty finite)
+next
+  case True
+  obtain R::\<open>(bracket \<times> ('n \<times> ('n, 't) sym list) \<times> version) list set\<close> and h and \<Gamma> where reg_R: \<open>(regular R)\<close> and L_minus_eq: \<open>(L-{[]} = image h (R \<inter> dyck_language \<Gamma>))\<close> and hom_h: \<open>hom h\<close>  by (metis L_def chomsky_schuetzenberger_not_empty finite)
+  then have reg_R_union: \<open>regular( R \<union> {[]})\<close> by (meson regular_Un regular_nullstr)
+  have \<open>[] = h([])\<close> using hom_def hom_h by metis
+  moreover have \<open>[] \<in> dyck_language \<Gamma>\<close> by fastforce
+  ultimately have \<open>[] \<in> h ` ((R \<union> {[]}) \<inter> dyck_language \<Gamma>)\<close> by blast
+  with True L_minus_eq have \<open>L = h ` ((R \<union> {[]}) \<inter> dyck_language \<Gamma>)\<close> using \<open>[] \<in> dyck_language \<Gamma>\<close> by auto
+  then show ?thesis using reg_R_union hom_h by blast
+qed
+
+
 
 
 
